%\chapterimage{head2.png} % Chapter heading image
\appendix{Integrals}
\label{appendix1.Integrals}

\ifpdf
\graphicspath{{Appendix1/figs/}}
\else
\graphicspath{{Appendix1/figs/}}
\fi

\begin{equation}
	\int_{-\infty}^{\infty} e^{-x^2} dx = \sqrt{\pi}
\end{equation}
proof:\\
let,
\begin{equation}
	I = \int_{-\infty}^{\infty} e^{-x^2} dx 
\end{equation}
then
\begin{eqnarray}
	I^2 = \int_{-\infty}^{\infty}\int_{-\infty}^{\infty} e^{-(x^2+y^2)} dx dy
\end{eqnarray}
using $r^2 = x^2 + y^2$ since
\begin{eqnarray}
	x &= r \cos \theta \\
	y &= r \sin \theta
\end{eqnarray}
we get 
\begin{eqnarray}
	I^2 
	&= \int_{0}^{2 \pi}\int_{0}^{\infty} e^{-r^2} r dr d\theta \\
	&= 2 \pi \int_{0}^{\infty} e^{-r^2} r dr
\end{eqnarray}
let $u = r^2$ therefore $rdr = du/2$
\begin{eqnarray}
I^2 
&=  \pi \int_{0}^{\infty} e^{-u} du \\
&=  \pi \left[\frac{e^{-u}}{-1} \right]_{0}^{\infty} \\
&= \pi \left[0 - (-1)\right] \\
&= \pi
\end{eqnarray}
therefore $I=\sqrt{\pi}$\\
\textbf{another}\\
\begin{eqnarray}
I = \int_{-\infty}^{\infty} dx \  e^{-\left(b^2 x^2 + a x\right)}
\end{eqnarray}
Notice that $\left(b^2 x^2 + a x\right) = (b x + \frac{a}{2 b})^2 - \frac{a^2}{4b^2}$
\begin{eqnarray}
I = e^{a^2/4b^2}\int_{-\infty}^{\infty} dx\ e^{-(b x + \frac{a}{2 b})^2}
\end{eqnarray}
let $z = b x + \frac{a}{2 b}$ thus $dz = b dx$
\begin{eqnarray}
I 
&= e^{a^2/4b^2} \frac{1}{b} \int_{-\infty}^{\infty} dz\  e^{-z^2} \\
&= e^{a^2/4b^2} \frac{\sqrt{\pi}}{b}
\end{eqnarray}